prop.dfy
@@ -1,0 +1,36 @@
+module Prop {
+    predicate shorterThan(sub: seq<int>, sequence: seq<int>)
+    {
+        |sub| < |sequence|
+    }
+
+    predicate strictlyIncreasing(a: array<nat>) 
+    reads a
+    {
+        forall i, j :: 0 <= i < j < a.Length ==> a[i] < a[j]
+    }
+
+    predicate increasing(a: array<nat>) 
+    reads a
+    {
+        forall i, j :: 0 <= i < j < a.Length ==> a[i] <= a[j]
+    }
+
+    predicate subsetOf(x: array<int>, y: array<int>)
+    reads x, y
+    {
+        multiset(y[..]) * multiset(x[..]) == multiset(x[..])
+    }
+
+    predicate boundedElements(x: array<nat>) 
+    reads x
+    {
+        forall i :: 0 <= i < x.Length ==> 0 < x[i] <= x.Length
+    }
+
+    predicate uniformArray(x: array<nat>) 
+    reads x
+    {
+        forall i, j :: 0 <= i < j < x.Length ==> x[i] == x[j]
+    }
+}
